src/HOL/IMP/Collecting.thy
@@ -11,16 +11,21 @@ notation
   bot ("\<bottom>") and
   top ("\<top>")
 
-fun Step :: "(vname \<Rightarrow> aexp \<Rightarrow> 'a \<Rightarrow> 'a::sup) \<Rightarrow> (bexp \<Rightarrow> 'a \<Rightarrow> 'a) \<Rightarrow> 'a \<Rightarrow> 'a acom \<Rightarrow> 'a acom" where
-"Step f g S (SKIP {Q}) = (SKIP {S})" |
-"Step f g S (x ::= e {Q}) =
+context
+  fixes f :: "vname \<Rightarrow> aexp \<Rightarrow> 'a \<Rightarrow> 'a::sup"
+  fixes g :: "bexp \<Rightarrow> 'a \<Rightarrow> 'a"
+begin
+fun Step :: "'a \<Rightarrow> 'a acom \<Rightarrow> 'a acom" where
+"Step S (SKIP {Q}) = (SKIP {S})" |
+"Step S (x ::= e {Q}) =
   x ::= e {f x e S}" |
-"Step f g S (C1; C2) = Step f g S C1; Step f g (post C1) C2" |
-"Step f g S (IF b THEN {P1} C1 ELSE {P2} C2 {Q}) =
-  IF b THEN {g b S} Step f g P1 C1 ELSE {g (Not b) S} Step f g P2 C2
+"Step S (C1; C2) = Step S C1; Step (post C1) C2" |
+"Step S (IF b THEN {P1} C1 ELSE {P2} C2 {Q}) =
+  IF b THEN {g b S} Step P1 C1 ELSE {g (Not b) S} Step P2 C2
   {post C1 \<squnion> post C2}" |
-"Step f g S ({I} WHILE b DO {P} C {Q}) =
-  {S \<squnion> post C} WHILE b DO {g b I} Step f g P C {g (Not b) I}"
+"Step S ({I} WHILE b DO {P} C {Q}) =
+  {S \<squnion> post C} WHILE b DO {g b I} Step P C {g (Not b) I}"
+end
 
 lemma strip_Step[simp]: "strip(Step f g S C) = strip C"
 by(induct C arbitrary: S) auto
@@ -33,33 +38,8 @@ subsubsection "Annotated commands as a complete lattice"
 instantiation acom :: (order) order
 begin
 
-fun less_eq_acom :: "('a::order)acom \<Rightarrow> 'a acom \<Rightarrow> bool" where
-"(SKIP {P}) \<le> (SKIP {P'}) = (P \<le> P')" |
-"(x ::= e {P}) \<le> (x' ::= e' {P'}) = (x=x' \<and> e=e' \<and> P \<le> P')" |
-"(C1;C2) \<le> (C1';C2') = (C1 \<le> C1' \<and> C2 \<le> C2')" |
-"(IF b THEN {P1} C1 ELSE {P2} C2 {Q}) \<le> (IF b' THEN {P1'} C1' ELSE {P2'} C2' {Q'}) =
-  (b=b' \<and> P1 \<le> P1' \<and> C1 \<le> C1' \<and> P2 \<le> P2' \<and> C2 \<le> C2' \<and> Q \<le> Q')" |
-"({I} WHILE b DO {P} C {Q}) \<le> ({I'} WHILE b' DO {P'} C' {Q'}) =
-  (b=b' \<and> C \<le> C' \<and> I \<le> I' \<and> P \<le> P' \<and> Q \<le> Q')" |
-"less_eq_acom _ _ = False"
-
-lemma SKIP_le: "SKIP {S} \<le> c \<longleftrightarrow> (\<exists>S'. c = SKIP {S'} \<and> S \<le> S')"
-by (cases c) auto
-
-lemma Assign_le: "x ::= e {S} \<le> c \<longleftrightarrow> (\<exists>S'. c = x ::= e {S'} \<and> S \<le> S')"
-by (cases c) auto
-
-lemma Seq_le: "C1;C2 \<le> C \<longleftrightarrow> (\<exists>C1' C2'. C = C1';C2' \<and> C1 \<le> C1' \<and> C2 \<le> C2')"
-by (cases C) auto
-
-lemma If_le: "IF b THEN {p1} C1 ELSE {p2} C2 {S} \<le> C \<longleftrightarrow>
-  (\<exists>p1' p2' C1' C2' S'. C = IF b THEN {p1'} C1' ELSE {p2'} C2' {S'} \<and>
-     p1 \<le> p1' \<and> p2 \<le> p2' \<and> C1 \<le> C1' \<and> C2 \<le> C2' \<and> S \<le> S')"
-by (cases C) auto
-
-lemma While_le: "{I} WHILE b DO {p} C {P} \<le> W \<longleftrightarrow>
-  (\<exists>I' p' C' P'. W = {I'} WHILE b DO {p'} C' {P'} \<and> C \<le> C' \<and> p \<le> p' \<and> I \<le> I' \<and> P \<le> P')"
-by (cases W) auto
+definition less_eq_acom :: "('a::order)acom \<Rightarrow> 'a acom \<Rightarrow> bool" where
+"C1 \<le> C2 \<longleftrightarrow> strip C1 = strip C2 \<and> (\<forall>p<size(annos C1). anno C1 p \<le> anno C2 p)"
 
 definition less_acom :: "'a acom \<Rightarrow> 'a acom \<Rightarrow> bool" where
 "less_acom x y = (x \<le> y \<and> \<not> y \<le> x)"
@@ -68,101 +48,64 @@ instance
 proof
   case goal1 show ?case by(simp add: less_acom_def)
 next
-  case goal2 thus ?case by (induct x) auto
+  case goal2 thus ?case by(auto simp: less_eq_acom_def)
 next
-  case goal3 thus ?case
-  apply(induct x y arbitrary: z rule: less_eq_acom.induct)
-  apply (auto intro: le_trans simp: SKIP_le Assign_le Seq_le If_le While_le)
-  done
+  case goal3 thus ?case by(fastforce simp: less_eq_acom_def size_annos)
 next
   case goal4 thus ?case
-  apply(induct x y rule: less_eq_acom.induct)
-  apply (auto intro: le_antisym)
-  done
+    by(fastforce simp: le_antisym less_eq_acom_def size_annos
+         eq_acom_iff_strip_anno)
 qed
 
 end
 
-text_raw{*\snip{subadef}{2}{1}{% *}
-fun sub\<^isub>1 :: "'a acom \<Rightarrow> 'a acom" where
-"sub\<^isub>1(C\<^isub>1;C\<^isub>2) = C\<^isub>1" |
-"sub\<^isub>1(IF b THEN {P\<^isub>1} C\<^isub>1 ELSE {P\<^isub>2} C\<^isub>2 {Q}) = C\<^isub>1" |
-"sub\<^isub>1({I} WHILE b DO {P} C {Q}) = C"
-text_raw{*}%endsnip*}
+lemma less_eq_acom_annos:
+  "C1 \<le> C2 \<longleftrightarrow> strip C1 = strip C2 \<and> list_all2 (op \<le>) (annos C1) (annos C2)"
+by(auto simp add: less_eq_acom_def anno_def list_all2_conv_all_nth size_annos_same2)
 
-text_raw{*\snip{subbdef}{1}{1}{% *}
-fun sub\<^isub>2 :: "'a acom \<Rightarrow> 'a acom" where
-"sub\<^isub>2(C\<^isub>1;C\<^isub>2) = C\<^isub>2" |
-"sub\<^isub>2(IF b THEN {P\<^isub>1} C\<^isub>1 ELSE {P\<^isub>2} C\<^isub>2 {Q}) = C\<^isub>2"
-text_raw{*}%endsnip*}
+lemma SKIP_le[simp]: "SKIP {S} \<le> c \<longleftrightarrow> (\<exists>S'. c = SKIP {S'} \<and> S \<le> S')"
+by (cases c) (auto simp:less_eq_acom_def anno_def)
 
-text_raw{*\snip{annoadef}{1}{1}{% *}
-fun anno\<^isub>1 :: "'a acom \<Rightarrow> 'a" where
-"anno\<^isub>1(IF b THEN {P\<^isub>1} C\<^isub>1 ELSE {P\<^isub>2} C\<^isub>2 {Q}) = P\<^isub>1" |
-"anno\<^isub>1({I} WHILE b DO {P} C {Q}) = I"
-text_raw{*}%endsnip*}
+lemma Assign_le[simp]: "x ::= e {S} \<le> c \<longleftrightarrow> (\<exists>S'. c = x ::= e {S'} \<and> S \<le> S')"
+by (cases c) (auto simp:less_eq_acom_def anno_def)
 
-text_raw{*\snip{annobdef}{1}{2}{% *}
-fun anno\<^isub>2 :: "'a acom \<Rightarrow> 'a" where
-"anno\<^isub>2(IF b THEN {P\<^isub>1} C\<^isub>1 ELSE {P\<^isub>2} C\<^isub>2 {Q}) = P\<^isub>2" |
-"anno\<^isub>2({I} WHILE b DO {P} C {Q}) = P"
-text_raw{*}%endsnip*}
+lemma Seq_le[simp]: "C1;C2 \<le> C \<longleftrightarrow> (\<exists>C1' C2'. C = C1';C2' \<and> C1 \<le> C1' \<and> C2 \<le> C2')"
+apply (cases C)
+apply(auto simp: less_eq_acom_annos list_all2_append size_annos_same2)
+done
 
-fun merge :: "com \<Rightarrow> 'a acom set \<Rightarrow> 'a set acom" where
-"merge com.SKIP M = (SKIP {post ` M})" |
-"merge (x ::= a) M = (x ::= a {post ` M})" |
-"merge (c1;c2) M =
-  merge c1 (sub\<^isub>1 ` M); merge c2 (sub\<^isub>2 ` M)" |
-"merge (IF b THEN c1 ELSE c2) M =
-  IF b THEN {anno\<^isub>1 ` M} merge c1 (sub\<^isub>1 ` M) ELSE {anno\<^isub>2 ` M} merge c2 (sub\<^isub>2 ` M)
-  {post ` M}" |
-"merge (WHILE b DO c) M =
- {anno\<^isub>1 ` M}
- WHILE b DO {anno\<^isub>2 ` M} merge c (sub\<^isub>1 ` M)
- {post ` M}"
+lemma If_le[simp]: "IF b THEN {p1} C1 ELSE {p2} C2 {S} \<le> C \<longleftrightarrow>
+  (\<exists>p1' p2' C1' C2' S'. C = IF b THEN {p1'} C1' ELSE {p2'} C2' {S'} \<and>
+     p1 \<le> p1' \<and> p2 \<le> p2' \<and> C1 \<le> C1' \<and> C2 \<le> C2' \<and> S \<le> S')"
+apply (cases C)
+apply(auto simp: less_eq_acom_annos list_all2_append size_annos_same2)
+done
+
+lemma While_le[simp]: "{I} WHILE b DO {p} C {P} \<le> W \<longleftrightarrow>
+  (\<exists>I' p' C' P'. W = {I'} WHILE b DO {p'} C' {P'} \<and> C \<le> C' \<and> p \<le> p' \<and> I \<le> I' \<and> P \<le> P')"
+apply (cases W)
+apply(auto simp: less_eq_acom_annos list_all2_append size_annos_same2)
+done
+
+lemma mono_post: "C \<le> C' \<Longrightarrow> post C \<le> post C'"
+using annos_ne[of C']
+by(auto simp: post_def less_eq_acom_def last_conv_nth[OF annos_ne] anno_def
+     dest: size_annos_same)
+
+definition Inf_acom :: "com \<Rightarrow> 'a::complete_lattice acom set \<Rightarrow> 'a acom" where
+"Inf_acom c M = annotate (\<lambda>p. INF C:M. anno C p) c"
 
 interpretation
-  Complete_Lattice "{C. strip C = c}" "map_acom Inter o (merge c)" for c
+  Complete_Lattice "{C. strip C = c}" "Inf_acom c" for c
 proof
-  case goal1
-  have "a:A \<Longrightarrow> map_acom Inter (merge (strip a) A) \<le> a"
-  proof(induction a arbitrary: A)
-    case Seq from Seq.prems show ?case by(force intro!: Seq.IH)
-  next
-    case If from If.prems show ?case by(force intro!: If.IH)
-  next
-    case While from While.prems show ?case by(force intro!: While.IH)
-  qed force+
-  with goal1 show ?case by auto
+  case goal1 thus ?case
+    by(auto simp: Inf_acom_def less_eq_acom_def size_annos intro:INF_lower)
 next
-  case goal2
-  thus ?case
-  proof(simp, induction b arbitrary: c A)
-    case SKIP thus ?case by (force simp:SKIP_le)
-  next
-    case Assign thus ?case by (force simp:Assign_le)
-  next
-    case Seq from Seq.prems show ?case by(force intro!: Seq.IH simp:Seq_le)
-  next
-    case If from If.prems show ?case by (force simp: If_le intro!: If.IH)
-  next
-    case While from While.prems show ?case by(fastforce simp: While_le intro: While.IH)
-  qed
+  case goal2 thus ?case
+    by(auto simp: Inf_acom_def less_eq_acom_def size_annos intro:INF_greatest)
 next
-  case goal3
-  have "strip(merge c A) = c"
-  proof(induction c arbitrary: A)
-    case Seq from Seq.prems show ?case by (fastforce simp: strip_eq_Seq subset_iff intro!: Seq.IH)
-  next
-    case If from If.prems show ?case by (fastforce intro!: If.IH simp: strip_eq_If)
-  next
-    case While from While.prems show ?case by(fastforce intro: While.IH simp: strip_eq_While)
-  qed auto
-  thus ?case by auto
+  case goal3 thus ?case by(auto simp: Inf_acom_def)
 qed
-
-lemma le_post: "c \<le> d \<Longrightarrow> post c \<le> post d"
-by(induction c d rule: less_eq_acom.induct) auto
 
 
 subsubsection "Collecting semantics"
@@ -176,17 +119,21 @@ lemma mono2_Step: fixes C1 C2 :: "'a::semilattice_sup acom"
   assumes "!!x e S1 S2. S1 \<le> S2 \<Longrightarrow> f x e S1 \<le> f x e S2"
           "!!b S1 S2. S1 \<le> S2 \<Longrightarrow> g b S1 \<le> g b S2"
   shows "C1 \<le> C2 \<Longrightarrow> S1 \<le> S2 \<Longrightarrow> Step f g S1 C1 \<le> Step f g S2 C2"
-proof(induction C1 C2 arbitrary: S1 S2 rule: less_eq_acom.induct)
-  case 2 thus ?case by (fastforce simp: assms(1))
+proof(induction S1 C1 arbitrary: C2 S2 rule: Step.induct)
+  case 1 thus ?case by(auto)
 next
-  case 3 thus ?case by(simp add: le_post)
+  case 2 thus ?case by (auto simp: assms(1))
+next
+  case 3 thus ?case by(auto simp: mono_post)
 next
   case 4 thus ?case
-    by(simp add: subset_iff assms(2)) (metis le_post le_supI1 le_supI2)
+    by(auto simp: subset_iff assms(2))
+      (metis mono_post le_supI1 le_supI2)+
 next
   case 5 thus ?case
-    by(simp add: subset_iff assms(2)) (metis le_post le_supI1 le_supI2)
-qed auto
+    by(auto simp: subset_iff assms(2))
+      (metis mono_post le_supI1 le_supI2)+
+qed
 
 lemma mono2_step: "C1 \<le> C2 \<Longrightarrow> S1 \<subseteq> S2 \<Longrightarrow> step S1 C1 \<le> step S2 C2"
 unfolding step_def by(rule mono2_Step) auto
@@ -211,31 +158,34 @@ by(simp add: CS_def index_lfp[simplified])
 
 subsubsection "Relation to big-step semantics"
 
-lemma post_merge: "\<forall> c' \<in> M. strip c' = c \<Longrightarrow> post (merge c M) = post ` M"
-proof(induction c arbitrary: M)
-  case (Seq c1 c2)
-  have "post ` M = post ` sub\<^isub>2 ` M" using Seq.prems by (force simp: strip_eq_Seq)
-  moreover have "\<forall> c' \<in> sub\<^isub>2 ` M. strip c' = c2" using Seq.prems by (auto simp: strip_eq_Seq)
-  ultimately show ?case using Seq.IH(2)[of "sub\<^isub>2 ` M"] by simp
-qed simp_all
+lemma asize_nz: "asize(c::com) \<noteq> 0"
+by (metis length_0_conv length_annos_annotate annos_ne)
 
+lemma post_Inf_acom:
+  "\<forall>C\<in>M. strip C = c \<Longrightarrow> post (Inf_acom c M) = \<Inter>(post ` M)"
+apply(subgoal_tac "\<forall>C\<in>M. size(annos C) = asize c")
+ apply(simp add: post_anno_asize Inf_acom_def asize_nz neq0_conv[symmetric])
+apply(simp add: size_annos)
+done
 
 lemma post_lfp: "post(lfp c f) = (\<Inter>{post C|C. strip C = c \<and> f C \<le> C})"
-by(auto simp add: lfp_def post_merge)
+by(auto simp add: lfp_def post_Inf_acom)
 
 lemma big_step_post_step:
   "\<lbrakk> (c, s) \<Rightarrow> t;  strip C = c;  s \<in> S;  step S C \<le> C \<rbrakk> \<Longrightarrow> t \<in> post C"
 proof(induction arbitrary: C S rule: big_step_induct)
-  case Skip thus ?case by(auto simp: strip_eq_SKIP step_def)
+  case Skip thus ?case by(auto simp: strip_eq_SKIP step_def post_def)
 next
-  case Assign thus ?case by(fastforce simp: strip_eq_Assign step_def)
+  case Assign thus ?case
+    by(fastforce simp: strip_eq_Assign step_def post_def)
 next
-  case Seq thus ?case by(fastforce simp: strip_eq_Seq step_def)
+  case Seq thus ?case
+    by(fastforce simp: strip_eq_Seq step_def post_def last_append annos_ne)
 next
-  case IfTrue thus ?case apply(auto simp: strip_eq_If step_def)
+  case IfTrue thus ?case apply(auto simp: strip_eq_If step_def post_def)
     by (metis (lifting,full_types) mem_Collect_eq set_mp)
 next
-  case IfFalse thus ?case apply(auto simp: strip_eq_If step_def)
+  case IfFalse thus ?case apply(auto simp: strip_eq_If step_def post_def)
     by (metis (lifting,full_types) mem_Collect_eq set_mp)
 next
   case (WhileTrue b s1 c' s2 s3)
@@ -243,7 +193,7 @@ next
     by(auto simp: strip_eq_While)
   from WhileTrue.prems(3) `C = _`
   have "step P C' \<le> C'"  "{s \<in> I. bval b s} \<le> P"  "S \<le> I"  "step (post C') C \<le> C"
-    by (auto simp: step_def)
+    by (auto simp: step_def post_def)
   have "step {s \<in> I. bval b s} C' \<le> C'"
     by (rule order_trans[OF mono2_step[OF order_refl `{s \<in> I. bval b s} \<le> P`] `step P C' \<le> C'`])
   have "s1: {s:I. bval b s}" using `s1 \<in> S` `S \<subseteq> I` `bval b s1` by auto
@@ -251,7 +201,8 @@ next
   from WhileTrue.IH(2)[OF WhileTrue.prems(1) s2_in_post_C' `step (post C') C \<le> C`]
   show ?case .
 next
-  case (WhileFalse b s1 c') thus ?case by (force simp: strip_eq_While step_def)
+  case (WhileFalse b s1 c') thus ?case
+    by (force simp: strip_eq_While step_def post_def)
 qed
 
 lemma big_step_lfp: "\<lbrakk> (c,s) \<Rightarrow> t;  s \<in> S \<rbrakk> \<Longrightarrow> t \<in> post(lfp c (step S))"
